src/two/new-wsat.v
@@ -317,6 +317,71 @@ Proof.
   iFrame "HI". iFrame "HiP2". iLeft. by rewrite /ownD; iFrame.
 Qed.
 
+Lemma ownI_alloc_and_simultaneous_own_alloc_ns (P : positive -> iProp Σ) `{ing : !inG Σ A} (a: A) (from: coPset) (inf: ¬set_finite from) :
+  (✓ a) ->
+  wsat ==∗ ∃ i, ⌜ i ∈ from ⌝ ∗ (▷ P i -∗ wsat) ∗ ownI i (P i) ∗ own i a.
+Proof.
+  intro valid_a.
+  iIntros "Hw". rewrite /wsat -!lock.
+  iDestruct "Hw" as (I) "[Hw [HI Hd]]".
+  
+  iMod (own_alloc_strong a (λ i , i ∉ dom (gset gname) I ∧ i ∈ from)) as "ow".
+  {
+    unfold pred_infinite.
+    intro xs.
+    assert (set_infinite (from ∖ dom coPset I ∖ list_to_set xs)) as infi.
+    - apply difference_infinite.
+      + apply difference_infinite.
+        * rewrite coPset_infinite_finite. trivial.
+        * apply dom_finite.
+      + apply list_to_set_finite.
+    - exists (coPpick (from ∖ dom coPset I ∖ list_to_set xs)).
+      assert (
+          (coPpick (from ∖ dom coPset I ∖ list_to_set xs))
+          ∈
+          (from ∖ dom coPset I ∖ list_to_set xs)
+      ) as IN. { apply coPpick_elem_of. rewrite <- coPset_infinite_finite. trivial. }
+      generalize IN.
+      rewrite elem_of_difference.
+      rewrite elem_of_difference.
+      rewrite elem_of_list_to_set.
+      rewrite elem_of_dom.
+      rewrite elem_of_dom.
+      intuition.
+  }
+  { trivial. }
+  
+  iDestruct "ow" as (i) "[%ni ow]".
+  destruct ni as [ni in_from].
+  
+  assert (I !! i = None) as HIi by (apply not_in_dom_to_none; trivial).
+  
+  assert (i ∈ (⊤ ∖ gmap_dom_coPset I)) as in_comp. { apply not_in_dom. trivial. }
+  have du := diff_union _ _ in_comp.
+  rewrite du.
+  
+  iDestruct (ownD_op with "Hd") as "[Hd HE]". { set_solver. }
+  
+  iMod (own_update with "Hw") as "[Hw HiP]".
+  { eapply (gmap_view_alloc _ i DfracDiscarded); last done.
+    by rewrite /= lookup_fmap HIi. }
+  
+  iModIntro. iExists i.
+  
+  rewrite /ownI.
+  iDestruct (bi.persistent_sep_dup with "HiP") as "[HiP HiP2]".
+  iFrame "HiP". iFrame "ow".
+  iSplitL "". { iPureIntro. trivial. }
+  iIntros "laterp".
+  iExists (<[i:=P i]>I); iSplitL "Hw".
+  { by rewrite fmap_insert. }
+  
+  rewrite diff_domm_inserted. iFrame "Hd".
+  
+  iApply (big_sepM_insert _ I); first done.
+  iFrame "HI". iFrame "HiP2". iLeft. by rewrite /ownD; iFrame.
+Qed.
+
 (*
 Lemma ownI_alloc_open_and_simultaneous_own_alloc (P : positive -> iProp Σ) `{ing : !inG Σ A} (a: A) :
   (✓ a) ->
